src/matroid/loop.lean
@@ -15,112 +15,150 @@ open set
 
 namespace matroid
 
-lemma loop_def :
-  M.loop e ↔ M.circuit {e} :=
-iff.rfl
+/- ### Loops -/
 
-lemma loop.circuit (he : M.loop e) :
-  M.circuit {e} :=
-he
+lemma loop_iff_mem_cl_empty : M.loop e ↔ e ∈ M.cl ∅ := iff.rfl 
 
-lemma loop.r (he : M.loop e) :
-  M.r {e} = 0 :=
+lemma cl_empty_eq_loops (M : matroid E) : M.cl ∅ = {e | M.loop e} := rfl 
+
+lemma loop_iff_dep : M.loop e ↔ ¬ M.indep {e} :=
+by rw [loop_iff_mem_cl_empty, iff_not_comm, M.empty_indep.not_mem_cl_iff, mem_empty_iff_false, 
+    not_false_iff, true_and, insert_emptyc_eq]
+
+lemma loop_iff_circuit : M.loop e ↔ M.circuit {e} := 
 begin
- have h := he.circuit.card,
- rwa [ncard_singleton, self_eq_add_left] at h,
-end
+  simp_rw [circuit, loop_iff_dep, iff_self_and, ssubset_singleton_iff, forall_eq], 
+  exact λ _, M.empty_indep, 
+end 
 
-lemma loop_iff_r :
-  M.loop e ↔ M.r {e} = 0 :=
+lemma loop_iff_r : M.loop e ↔ M.r {e} = 0 :=
 begin
-  refine ⟨loop.r, λ h, _⟩,
-  rw [loop_def, circuit_def, ←r_lt_card_iff_dep, h, ncard_singleton],
-  refine ⟨zero_lt_one, λ I hI, _⟩,
-  rw [ssubset_singleton_iff.mp hI],
-  apply empty_indep,
-end
+  rw [loop_iff_dep, indep_iff_r_eq_card, ncard_singleton],
+  refine ⟨λ h, nat.eq_zero_of_le_zero (nat.lt_succ_iff.mp _), 
+    λ h h', (nat.zero_ne_one (h.symm.trans h'))⟩,
+  convert (M.r_le_card {e}).lt_of_ne (by rwa ncard_singleton),
+  rw ncard_singleton,  
+end 
 
-lemma loop_iff_not_mem_base_forall :
-  M.loop e ↔ ∀ B, M.base B → e ∉ B :=
-begin
-  refine ⟨λ h B hB heB, h.circuit.dep (hB.indep.subset (singleton_subset_iff.mpr heB)),
-    λ h, _⟩,
-  refine ⟨λ h_ind, _,λ I hI, _⟩,
-  { obtain ⟨B,hB⟩ := h_ind.exists_base_supset,
-    exact h _ hB.1 (singleton_subset_iff.mp hB.2)},
-  convert M.empty_indep,
-  rwa ssubset_singleton_iff at hI,
-end
+lemma loop.circuit (he : M.loop e) : M.circuit {e} := loop_iff_circuit.mp he 
 
-lemma loop_iff_dep :
-  M.loop e ↔ ¬M.indep {e} :=
-⟨circuit.dep, λ h, loop_iff_not_mem_base_forall.mpr
-  (λ B hB heB, h (hB.indep.subset (singleton_subset_iff.mpr heB)))⟩
+lemma loop.r (he : M.loop e) : M.r {e} = 0 := loop_iff_r.mp he 
 
-lemma nonloop_iff_indep :
-  (¬ M.loop e) ↔ M.indep {e} :=
-by rw [not_iff_comm, loop_iff_dep]
+lemma loop.mem_cl (he : M.loop e) (X : set E) : e ∈ M.cl X :=
+M.cl_mono (empty_subset _) he 
 
-lemma loop_iff_mem_cl_empty :
-  M.loop e ↔ e ∈ M.cl ∅ :=
-begin
-  rw [loop_iff_dep, not_iff_comm, not_mem_cl_iff_forall_insert_basis_insert],
-  split,
-  { rintro ⟨-,h⟩, simpa using (h ∅ M.empty_basis_empty).indep},
-  refine λ h, ⟨not_mem_empty _, λ I hI, _⟩,
-  rw ←basis_self_iff_indep at h,
-  rw basis_empty_iff at hI, subst hI,
-  convert h;
-  simp,
-end
+lemma loop.mem_flat (he : M.loop e) {F : set E} (hF : M.flat F) : e ∈ F :=
+by { have := he.mem_cl F, rwa hF.cl at this }
 
-lemma cl_empty_eq_loops (M : matroid E) :
-  M.cl ∅ = {e | M.loop e} :=
-by {simp_rw loop_iff_mem_cl_empty, refl}
-
-lemma loop.mem_cl (he : M.loop e) (X : set E) :
-  e ∈ M.cl X :=
-mem_of_mem_of_subset (loop_iff_mem_cl_empty.mp he) (M.cl_mono (empty_subset _))
-
-lemma loop.dep_of_mem (he : M.loop e) (h : e ∈ X) :
-  ¬M.indep X :=
+lemma loop.dep_of_mem (he : M.loop e) (h : e ∈ X) : ¬M.indep X :=
 λ hX, he.circuit.dep (hX.subset (singleton_subset_iff.mpr h))
 
-lemma loop.not_mem_indep (he : M.loop e) (hI : M.indep I) :
-  e ∉ I :=
+lemma loop.not_mem_indep (he : M.loop e) (hI : M.indep I) : e ∉ I :=
 λ h, he.dep_of_mem h hI
 
-lemma indep.nonloop_of_mem (hI : M.indep I) (h : e ∈ I) :
-  ¬ M.loop e :=
-λ he, (he.not_mem_indep hI) h
-
-lemma mem_nonloops_iff_not_loop :
-  e ∈ M.nonloops ↔ ¬M.loop e :=
-by rw [nonloops, mem_compl_iff, loop_iff_mem_cl_empty]
-
-lemma indep.disjoint_loops (hI : M.indep I) :
-  disjoint I (M.cl ∅) :=
-begin
-  rw [cl_empty_eq_loops],
-  by_contra' h,
-  obtain ⟨e,he⟩ := not_disjoint_iff.mp h,
-  exact he.2.not_mem_indep hI he.1,
-end
-
-lemma nonloop_iff_r :
-  ¬M.loop e ↔ M.r {e} = 1 :=
-by rw [nonloop_iff_indep, indep_iff_r_eq_card, ncard_singleton]
-
-lemma loop.eq_of_circuit_mem (he : M.loop e) (hC : M.circuit C) (h : e ∈ C) :
-  C = {e} :=
+lemma loop.eq_of_circuit_mem (he : M.loop e) (hC : M.circuit C) (h : e ∈ C) : C = {e} :=
 by rw he.circuit.eq_of_subset_circuit hC (singleton_subset_iff.mpr h)
 
-lemma coloop_def :
-  M.coloop e ↔ ∀ B, M.base B → e ∈ B :=
-iff.rfl
+lemma indep.disjoint_loops (hI : M.indep I) : disjoint I (M.cl ∅) :=
+by_contra (λ h, let ⟨e,⟨heI,he⟩⟩ := not_disjoint_iff.mp h in loop.not_mem_indep he hI heI)
 
-lemma coloop.r_compl_add_one (he : M.coloop e) :
-  M.r {e}ᶜ + 1 = M.rk :=
+lemma cl_eq_loops_of_subset (h : X ⊆ M.cl ∅) : M.cl X = M.cl ∅ :=
+(cl_subset_cl_of_subset_cl h).antisymm (M.cl_mono (empty_subset _))
+
+lemma loop.cl (he : M.loop e) : M.cl {e} = M.cl ∅ :=
+cl_eq_loops_of_subset (singleton_subset_iff.mpr he)
+
+lemma r_eq_zero_iff_forall_loop : M.r X = 0 ↔ ∀ e ∈ X, M.loop e :=
+begin
+  refine ⟨λ h e he, loop_iff_r.mpr ((nat.zero_le _).antisymm' _), λ h, (nat.zero_le _).antisymm' _⟩,
+  { rw ←h, exact M.r_mono (singleton_subset_iff.mpr he) },
+  have h' := M.r_mono h, 
+  rwa [r_cl, r_empty] at h', 
+end 
+
+lemma r_zero_iff_subset_loops : M.r X = 0 ↔ X ⊆ M.cl ∅ := r_eq_zero_iff_forall_loop
+
+/- ### Nonloops -/
+
+lemma nonloop_iff_not_loop : M.nonloop e ↔ ¬ M.loop e := iff.rfl 
+
+lemma loop_or_nonloop (M : matroid E) (e : E) : M.loop e ∨ M.nonloop e := em _ 
+
+lemma nonloop_iff_indep : M.nonloop e ↔ M.indep {e} := by rw [nonloop, not_iff_comm, loop_iff_dep]
+
+lemma nonloop_iff_r : M.nonloop e ↔ M.r {e} = 1 :=
+by rw [nonloop_iff_indep, indep_iff_r_eq_card, ncard_singleton]
+
+lemma nonloop.indep (h : M.nonloop e) : M.indep {e} := nonloop_iff_indep.mp h 
+
+lemma nonloop.r (he : M.nonloop e) : M.r {e} = 1 := nonloop_iff_r.mp he 
+
+lemma indep.nonloop_of_mem (hI : M.indep I) (h : e ∈ I) : ¬ M.loop e := 
+λ he, (he.not_mem_indep hI) h
+
+lemma circuit.nonloop_of_mem_of_one_lt_card (hC : M.circuit C) (h : 1 < C.ncard) (he : e ∈ C) :
+  M.nonloop e :=
+nonloop_iff_not_loop.mpr (λ hlp, by simpa [hlp.eq_of_circuit_mem hC he] using h)
+
+lemma nonloop_of_not_mem_cl (h : e ∉ M.cl X) : M.nonloop e :=
+nonloop_iff_not_loop.mpr (λ he, h (he.mem_cl X))
+
+lemma nonloop.mem_cl_singleton (he : M.nonloop e) (hef : e ∈ M.cl {f}) : f ∈ M.cl {e} :=
+begin
+  refine (M.loop_or_nonloop f).elim (λ hf, hf.mem_cl _) (λ hf, _), 
+  rw [he.indep.mem_cl_iff, mem_singleton_iff], 
+  rwa [hf.indep.mem_cl_iff, mem_singleton_iff, eq_comm, pair_comm] at hef, 
+end 
+
+lemma nonloop.mem_cl_comm (he : M.nonloop e) (hf : M.nonloop f) : f ∈ M.cl {e} ↔ e ∈ M.cl {f} :=
+⟨hf.mem_cl_singleton, he.mem_cl_singleton⟩ 
+
+lemma nonloop.nonloop_of_mem_cl (he : M.nonloop e) (hef : e ∈ M.cl {f}) : M.nonloop f :=
+λ hf, he (by rwa [hf.cl] at hef)
+  
+lemma nonloop.cl_eq_of_mem_cl (he : M.nonloop e) (hef : e ∈ M.cl {f}) : M.cl {e} = M.cl {f} :=
+begin
+  ext x, 
+  obtain (hx | hx) := M.loop_or_nonloop x, 
+  { exact ⟨λ _, hx.mem_cl _, λ _, hx.mem_cl _⟩ },
+  refine ⟨λ h, _, λ h, he.mem_cl_singleton _⟩,
+  { rw [←singleton_subset_iff, ←cl_subset_cl_iff_subset_cl] at *,
+    exact h.trans hef },
+  have hfx := hx.mem_cl_singleton h, 
+  rw [←singleton_subset_iff, ←cl_subset_cl_iff_subset_cl] at *,
+  exact hef.trans hfx, 
+end 
+
+lemma nonloop.cl_eq_cl_iff_dep (he : M.nonloop e) : M.cl {e} = M.cl {f} ↔ e = f ∨ ¬ M.indep {e,f} := 
+begin
+  obtain (hf | hf) := M.loop_or_nonloop f, 
+  { rw hf.cl,  },
+  -- have h' := @indep.mem_cl_iff _ _ M {f} e, 
+  -- rw [mem_singleton_iff] at h', 
+  refine ⟨λ hef, _, _⟩,
+  { have hf : f ∈ M.cl {e}, by {rw hef, exact M.mem_cl_self f },
+    rw [pair_comm, eq_comm, ←mem_singleton_iff], 
+    exact he.indep.mem_cl_iff.mp hf},  
+  rintro (rfl | hdep), refl, 
+  apply he.cl_eq_of_mem_cl, 
+  
+  have := he.indep.mem_cl_iff, 
+
+end 
+
+-- lemma cl_singleton_eq_cl_singleton_iff :
+--   M.cl {e} = M.cl {f} ↔ (M.loop e ∧ M.loop f) ∨ (M.nonloop e ∧ M.nonloop f ∧ M.parallel ) 
+
+
+
+
+
+
+/- ### Coloops -/ 
+
+lemma coloop_def : M.coloop e ↔ ∀ B, M.base B → e ∈ B := iff.rfl
+
+lemma coloop.r_compl_add_one (he : M.coloop e) : M.r {e}ᶜ + 1 = M.rk :=
 begin
   obtain ⟨I,hI⟩ := M.exists_basis {e}ᶜ,
   obtain ⟨B, hIB, hB⟩ := hI.indep.subset_basis_of_subset (subset_univ I),
@@ -139,8 +177,7 @@ begin
   rw [←hI.r, hI.indep.r, ←hB.r, hB.indep.r, ncard_insert_of_not_mem heI],
 end
 
-lemma coloop_iff_r_compl_add_one_eq :
-  M.coloop e ↔ M.r {e}ᶜ + 1 = M.rk :=
+lemma coloop_iff_r_compl_add_one_eq : M.coloop e ↔ M.r {e}ᶜ + 1 = M.rk :=
 begin
   refine ⟨coloop.r_compl_add_one, λ h B hB, by_contra (λ h', _)⟩,
   rw ←subset_compl_singleton_iff at h',
@@ -149,8 +186,7 @@ begin
   simpa only [add_le_iff_nonpos_right, le_zero_iff, nat.one_ne_zero] using hB',
 end
 
-lemma coloop_iff_r_compl_lt :
-  M.coloop e ↔ M.r {e}ᶜ < M.rk :=
+lemma coloop_iff_r_compl_lt : M.coloop e ↔ M.r {e}ᶜ < M.rk :=
 begin
   refine ⟨λ h, _,λ h, _⟩,
   { rw ←h.r_compl_add_one, apply lt_add_one, },
@@ -160,12 +196,10 @@ begin
   rw [coloop_iff_r_compl_add_one_eq, eq_comm, rk, ←he, r_insert_eq_add_one_of_r_ne h.ne.symm],
 end
 
-lemma coloop.coe_r_compl (he : M.coloop e) :
-  (M.r {e}ᶜ : ℤ) = M.rk - 1 :=
+lemma coloop.coe_r_compl (he : M.coloop e) : (M.r {e}ᶜ : ℤ) = M.rk - 1 :=
 by simp [←he.r_compl_add_one]
 
-lemma coloop.not_mem_circuit (he : M.coloop e) (hC : M.circuit C) :
-  e ∉ C :=
+lemma coloop.not_mem_circuit (he : M.coloop e) (hC : M.circuit C) : e ∉ C :=
 begin
   intro heC,
   obtain ⟨B,hB, hCB⟩ := (hC.diff_singleton_indep heC).exists_base_supset,
@@ -174,20 +208,5 @@ begin
   exact hC.dep (hB.indep.subset h),
 end
 
-lemma cl_eq_loops_of_subset (h : X ⊆ M.cl ∅) :
-  M.cl X = M.cl ∅ :=
-(cl_subset_cl_of_subset_cl h).antisymm (M.cl_mono (empty_subset _))
-
-lemma r_zero_iff_subset_loops :
-  M.r X = 0 ↔ X ⊆ M.cl ∅ :=
-begin
-  obtain ⟨I, hI⟩ := M.exists_basis X,
-  rw [←hI.r, hI.indep.r, ncard_eq_zero, ←cl_subset_cl_iff_subset_cl, ←hI.cl,
-    cl_subset_cl_iff_subset_cl],
-  refine ⟨λ h, _,λ h, _⟩,
-  { rw h, exact empty_subset _},
-  have := disjoint_iff_inter_eq_empty.mp hI.indep.disjoint_loops,
-  rwa inter_eq_left_iff_subset.mpr h at this,
-end
 
 end matroid
